agree/agree_fullSyntax.sig
@@ -32,12 +32,54 @@ sig
   val mk_Sub : term * term -> term
   val mk_Array : term -> term
   val mk_Recd : term -> term
-
   val mk_stmt : term * term -> term
-
   val mk_output_data : term * term -> term
   val mk_output_event : term * term -> term
   val mk_output_event_data : term * term * term -> term
-
   val mk_component : (string * term) list -> term
+
+
+  val dest_Var : term -> term
+  val dest_IntLit : term -> term
+  val dest_BoolLit : term -> term
+  val dest_Add : term -> term * term
+  val dest_And : term -> term * term
+  val dest_ArraySub : term -> term * term
+  val dest_Cond : term -> term * term * term
+  val dest_Div : term -> term * term
+  val dest_Sub : term -> term * term
+  val dest_Eq : term -> term * term
+  val dest_Fby : term -> term * term
+  val dest_Hist : term -> term
+  val dest_Iff : term -> term * term
+  val dest_Imp : term -> term * term
+  val dest_Leq : term -> term * term
+  val dest_Lt : term -> term * term
+  val dest_Mod : term -> term * term
+  val dest_Mult : term -> term * term
+  val dest_Not : term -> term
+  val dest_Or : term -> term * term
+  val dest_PortData : term -> term
+  val dest_PortEvent : term -> term
+  val dest_Pre : term -> term
+  val dest_RecdProj : term -> term * term
+  val dest_Array : term -> term
+  val dest_Recd : term -> term
+  val dest_stmt : term -> term * term
+  val dest_output_data : term -> term * term
+  val dest_output_event : term -> term * term
+  val dest_output_event_data : term -> term * term * term
+
+  datatype port
+    = Data of term
+    | Event_Only of term
+    | Event_Data of term * term
+
+  val dest_component
+    : term -> (string * string list) *
+              (string * (string * term) list) *
+              (string * (string * port) list) *
+              (string * term list) *
+              (string * term list)
+
 end
